removed multiset intersection as term constructor (establishes compatibility to AC1h wrt. AC1 multiset set)

theories/Problems/FMsetC.v
@@ -14,11 +14,16 @@
   The element (h^n 0) is represented by the natural number n.
 
   Terms t, u:
-    t, u ::= n : list nat | x : nat | t ⊍ u | t ⩀ u | h (t)
+    t, u ::= zero | t ⊍ u | h (t) | x : nat
     where x ranges over multiset variables
   
   Constraints:
     t ≐ u 
+
+  Term Interpretation:
+    φ(zero) = [0]
+    φ(t ⊍ u) = φ(t) ++ φ(u)
+    φ(h (t)) = map h (φ(t))
 
   FMsetC:
     Given a list (t₁ ≐ u₁),...,(tₙ ≐ uₙ) of constraints,
@@ -37,10 +42,9 @@ Import ListNotations.
 
 (* terms *)
 Inductive mset_term : Set :=
-  | mset_term_const : list nat -> mset_term
+  | mset_term_zero : mset_term
   | mset_term_var : nat -> mset_term
   | mset_term_plus : mset_term -> mset_term -> mset_term
-  | mset_term_cap : mset_term -> mset_term -> mset_term
   | mset_term_h : mset_term -> mset_term.
 
 (* list equality up to permutation *)
@@ -48,31 +52,12 @@ Definition mset_eq (A B : list nat) : Prop :=
   forall c, count_occ Nat.eq_dec A c = count_occ Nat.eq_dec B c.
 Notation "A ≡ B" := (mset_eq A B) (at level 65).
 
-(* removes the first occurrence of n in A, fails otherwise *)
-Fixpoint mset_try_remove (n : nat) (A : list nat) : option (list nat) :=
-  match A with
-  | [] => None
-  | (m :: A) => if Nat.eqb n m then Some A else option_map (cons m) (mset_try_remove n A)
-  end.
-
-(* multiset intersection *)
-Fixpoint mset_intersect (A B : list nat) : list nat :=
-  match A with
-  | [] => []
-  | (n :: A) => 
-    match mset_try_remove n B with
-    | None => mset_intersect A B
-    | Some(B) => n :: (mset_intersect A B)
-    end
-  end.
-
 (* evaluate an mset wrt. a valuation φ *)
 Fixpoint mset_sem (φ : nat -> list nat) (A : mset_term) : list nat :=
   match A with
-    | mset_term_const l => l
+    | mset_term_zero => [0]
     | mset_term_var x => φ x
     | mset_term_plus A B => (mset_sem φ A) ++ (mset_sem φ B)
-    | mset_term_cap A B => mset_intersect (mset_sem φ A) (mset_sem φ B)
     | mset_term_h A => map S (mset_sem φ A)
   end.
 
