theories/Reductions/H10UC_to_FMsetC.v
@@ -15,6 +15,7 @@
     [1] Paliath Narendran: Solving Linear Equations over Polynomial Semirings.
       LICS 1996: 466-472, doi: 10.1109/LICS.1996.561463
 *)
+
 Require Import ssreflect ssrbool ssrfun.
 Require Import Arith Psatz.
 Require Import List.
@@ -23,9 +24,8 @@ Import ListNotations.
 From Undecidability Require Import Problems.FMsetC Problems.H10UC Problems.Reduction.
 
 Notation "t ⊍ u" := (mset_term_plus t u) (at level 40).
-Notation "t ⩀ u" := (mset_term_cap t u) (at level 39).
 Notation "'h' t" := (mset_term_h t) (at level 38).
-Notation "• l" := (mset_term_const l) (at level 38, format "• l").
+Notation "•0" := mset_term_zero.
 
 Coercion mset_term_var : nat >-> mset_term.
 
@@ -36,13 +36,16 @@ Section Facts.
   Lemma measure_ind {X: Type} (f: X -> nat) (P: X -> Prop) : 
     (forall x, (forall y, f y < f x -> P y) -> P x) -> forall (x : X), P x.
   Proof.
-    apply : well_founded_ind.
-    apply : Wf_nat.well_founded_lt_compat. move => *. by eassumption.
+    apply: well_founded_ind.
+    apply: Wf_nat.well_founded_lt_compat. move=> *. by eassumption.
   Qed.
 
   (* transforms a goal (A -> B) -> C into goals A and B -> C *)
   Lemma unnest {A B C: Prop} : A -> (B -> C) -> (A -> B) -> C.
   Proof. auto. Qed.
+
+  Lemma unnest_t (X Y Z: Type): X -> (Y -> Z) -> (X -> Y) -> Z.
+  Proof. by auto. Qed.
 
   (* duplicates argument *)
   Lemma copy {A: Prop} : A -> A * A.
@@ -50,11 +53,7 @@ Section Facts.
 
 End Facts.
 
-Set Implicit Arguments.
-Set Maximal Implicit Insertion.
-
 Arguments mset_eq !A !B.
-Arguments mset_intersect !A !B.
 
 Definition mset_sat (φ : nat -> list nat) (l : FMsetC_PROBLEM) := 
   Forall (fun '(A, B) => (mset_sem φ A) ≡ (mset_sem φ B)) l.
@@ -138,6 +137,39 @@ Qed.
 (* usage: rewrite ? Forall_norm *)
 Definition Forall_norm := (@Forall_app_iff, @Forall_singleton_iff, @Forall_cons_iff, @Forall_nil_iff).
 
+(* Forall2 facts *)
+Lemma Forall2_nil_rE {X Y: Type} {P: X -> Y -> Prop} {A}: Forall2 P A [] -> A = [].
+Proof. move=> H. by inversion H. Qed.
+
+Lemma Forall2_nil_lE {X Y: Type} {P: X -> Y -> Prop} {A}: Forall2 P [] A -> A = [].
+Proof. move=> H. by inversion H. Qed.
+
+Lemma Forall2_lastP {X Y: Type} {P: X -> Y -> Prop} {A B a b}:
+  Forall2 P (A ++ [a]) (B ++ [b]) <-> Forall2 P A B /\ P a b.
+Proof. 
+  elim: A B => /=.
+    move=> B. constructor.
+      elim: B => /=.
+        move=> H. by inversion H.
+      move=> c B IH H. inversion H. subst.
+      have := Forall2_nil_lE ltac:(eassumption). by move /app_eq_nil => [_].
+    move=> [/Forall2_nil_lE ->] ? /=. by constructor.
+  move=> c A IH. elim=> /=.
+    constructor.
+      move=> H. inversion H. subst.
+      have := Forall2_nil_rE ltac:(eassumption). by move /app_eq_nil => [_].
+    by move=> [/Forall2_nil_rE].
+  move=> d B IH2. constructor.
+    move=> H. inversion H. subst. constructor.
+      constructor.
+        done.
+      have := iffLR (IH B) ltac:(eassumption). by case.
+    have := iffLR (IH B) ltac:(eassumption). by case.
+  move=> [H ?]. inversion H. subst. constructor.
+    done.
+  apply /IH. by constructor.
+Qed.
+
 (* seq facts *)
 Lemma seq_last start length : seq start (S length) = (seq start length) ++ [start + length].
 Proof.
@@ -153,6 +185,14 @@ Proof.
   move=> m IH. cbn. by f_equal.
 Qed.
 
+Lemma Forall_repeat {X: Type} {a} {A: list X} : Forall (fun b => a = b) A -> A = repeat a (length A).
+Proof.
+  elim: A.
+    done.
+  move=> b A IH. rewrite Forall_norm => [[? /IH ->]]. subst b.
+  cbn. by rewrite repeat_length.
+Qed.
+
 (* bijection between nat and nat * nat *)
 Module NatNat.
 
@@ -162,18 +202,16 @@ Definition big_sum (n : nat) : nat := nat_rec _ 0 (fun i m => m + (S i)) n.
 (* bijection from nat * nat to nat *)
 Definition nat2_to_nat '(x, y) : nat := (big_sum (x + y)) + y.
 
-Definition next_nat2 '(x, y) : nat * nat :=
-  if x is S x then (x, S y) else (S y, 0).
+Definition next_nat2 '(x, y) : nat * nat := if x is S x then (x, S y) else (S y, 0).
 
 (* bijection from nat to nat * nat *)
-Definition nat_to_nat2 (n : nat) : nat * nat :=
-  Nat.iter n next_nat2 (0, 0).
+Definition nat_to_nat2 (n : nat) : nat * nat := Nat.iter n next_nat2 (0, 0).
 
 Lemma nat_nat2_cancel : cancel nat2_to_nat nat_to_nat2.
 Proof.
   move=> a. move Hn: (nat2_to_nat a) => n.
   elim: n a Hn.
-    case; case=> [|a]; case=> [|b]=> /=; by [|lia].
+    case; case=> [|?]; case=> [|?]=> /=; by [|lia].
   move=> n IH [x y]. case: y => [|y] /=. case: x => [|x] //=.
   all: rewrite ? (Nat.add_0_r, Nat.add_succ_r); case.
     rewrite -/(nat2_to_nat (0, x)). by move /IH ->.
@@ -182,130 +220,124 @@ Qed.
 
 Lemma nat2_nat_cancel : cancel nat_to_nat2 nat2_to_nat.
 Proof.
-  elim => //=.
-  move => n. move : (nat_to_nat2 n) => [+ ?].
-  case => /= => [|?]; rewrite ? (Nat.add_0_r, Nat.add_succ_r) => /=; by lia.
+  elim=> //=.
+  move=> n. move: (nat_to_nat2 n) => [+ ?].
+  case=> /= => [|?]; rewrite ? (Nat.add_0_r, Nat.add_succ_r) => /=; by lia.
 Qed.
 
 End NatNat.
 
 (* eq facts *)
-  Lemma eq_refl {A} : A ≡ A.
-  Proof.
-    done.
-  Qed.
+Lemma eq_refl {A} : A ≡ A.
+Proof. done. Qed.
 
-  Lemma eq_eq {A B}: A = B -> A ≡ B.
-  Proof.
-    by move=> ->.
-  Qed.
+Lemma eq_eq {A B}: A = B -> A ≡ B.
+Proof. by move=> ->. Qed.
   
-  Lemma eq_symm {A B} : A ≡ B -> B ≡ A.
-  Proof.
-    by firstorder done.
-  Qed.
+Lemma eq_symm {A B} : A ≡ B -> B ≡ A.
+Proof. by firstorder done. Qed.
   
-  Lemma eq_in_iff {A B} : A ≡ B -> forall c, In c A <-> In c B.
-  Proof.
-    rewrite /mset_eq => H c. constructor=> Hc.
-    - have := iffLR (count_occ_In Nat.eq_dec A c) Hc.
-      move: (H c) => ->.
-      by move /(count_occ_In Nat.eq_dec B c).
-    - have := iffLR (count_occ_In Nat.eq_dec B c) Hc.
-      move: (H c) => <-.
-      by move /(count_occ_In Nat.eq_dec A c).
-  Qed.
+Lemma eq_in_iff {A B} : A ≡ B -> forall c, In c A <-> In c B.
+Proof.
+  rewrite /mset_eq => H c. constructor=> Hc.
+  - have := iffLR (count_occ_In Nat.eq_dec A c) Hc.
+    move: (H c) => ->.
+    by move /(count_occ_In Nat.eq_dec B c).
+  - have := iffLR (count_occ_In Nat.eq_dec B c) Hc.
+    move: (H c) => <-.
+    by move /(count_occ_In Nat.eq_dec A c).
+Qed.
 
-  Lemma eq_nilE {A} : [] ≡ A -> A = [].
-  Proof.
-    case: A.
-      done.
-    move=> a A /eq_in_iff /(_ a) /iffRL. apply: unnest.
-      by left.
+Lemma eq_nilE {A} : [] ≡ A -> A = [].
+Proof.
+  case: A.
     done.
-  Qed.
+  move=> a A /eq_in_iff /(_ a) /iffRL. apply: unnest.
+    by left.
+  done.
+Qed.
 
-  Lemma eq_trans {A B C} : A ≡ B -> B ≡ C -> A ≡ C.
-  Proof.
-    rewrite /mset_eq => + + c.
-    move=> /(_ c) + /(_ c).
-    by move=> -> ->.
-  Qed.
+Lemma eq_trans {A B C} : A ≡ B -> B ≡ C -> A ≡ C.
+Proof.
+  rewrite /mset_eq => + + c.
+  move=> /(_ c) + /(_ c).
+  by move=> -> ->.
+Qed.
 
-  Lemma eq_Forall_iff {A B} : A ≡ B -> forall P, (Forall P A <-> Forall P B).
-  Proof.
-    move /eq_in_iff => H P.
-    rewrite ? Forall_forall. constructor; by firstorder done.
-  Qed.
+Lemma eq_Forall_iff {A B} : A ≡ B -> forall P, (Forall P A <-> Forall P B).
+Proof.
+  move /eq_in_iff => H P.
+  rewrite ? Forall_forall. constructor; by firstorder done.
+Qed.
 
-  Lemma eq_lr {A B A' B'}:
-    A ≡ A' -> B ≡ B' -> (A ≡ B) <-> (A' ≡ B').
-  Proof.
-    move=> HA HB. constructor.
-    - move /eq_trans. move /(_ _ HB). 
-      move /(eq_trans _). by move /(_ _ (eq_symm HA)). 
-    - move /eq_trans. move /(_ _ (eq_symm HB)). 
-      move /(eq_trans _). by move /(_ _ HA).
-  Qed. 
+Lemma eq_lr {A B A' B'}:
+  A ≡ A' -> B ≡ B' -> (A ≡ B) <-> (A' ≡ B').
+Proof.
+  move=> HA HB. constructor.
+  - move /eq_trans. move /(_ _ HB). 
+    move /(eq_trans _). by move /(_ _ (eq_symm HA)). 
+  - move /eq_trans. move /(_ _ (eq_symm HB)). 
+    move /(eq_trans _). by move /(_ _ HA).
+Qed. 
 
-  Lemma eq_appI {A B A' B'} : A ≡ A' -> B ≡ B' -> A ++ B ≡ A' ++ B'.
-  Proof.
-    rewrite /mset_eq => + + c. move=> /(_ c) + /(_ c).
-    rewrite ? count_occ_app. by move=> -> ->.
-  Qed.
+Lemma eq_appI {A B A' B'} : A ≡ A' -> B ≡ B' -> A ++ B ≡ A' ++ B'.
+Proof.
+  rewrite /mset_eq => + + c. move=> /(_ c) + /(_ c).
+  rewrite ? count_occ_app. by move=> -> ->.
+Qed.
 
-  (* solves trivial multiset equalities *)
-  Ltac eq_trivial := 
-    move=> ?; rewrite ? (count_occ_app, count_occ_cons, count_occ_nil); unlock; by lia.
-      
-  Lemma eq_cons_iff {a A B} : (a :: A) ≡ (a :: B) <-> A ≡ B.
-  Proof.
-    rewrite /mset_eq. constructor.
-    all: move=> H c; move: {H}(H c); rewrite ? count_occ_cons ? in_cons_iff; unlock.
-    all: by rewrite Nat.add_cancel_l.
-  Qed.
+(* solves trivial multiset equalities *)
+Ltac eq_trivial := 
+  move=> ?; rewrite ? (count_occ_app, count_occ_cons, count_occ_nil); unlock; by lia.
+    
+Lemma eq_cons_iff {a A B} : (a :: A) ≡ (a :: B) <-> A ≡ B.
+Proof.
+  rewrite /mset_eq. constructor.
+  all: move=> H c; move: {H}(H c); rewrite ? count_occ_cons ? in_cons_iff; unlock.
+  all: by rewrite Nat.add_cancel_l.
+Qed.
 
-  Lemma eq_app_iff {A B C} : (A ++ B) ≡ (A ++ C) <-> B ≡ C.
-  Proof.
-    elim: A.
-      done.
-    move=> a A IH /=.
-    by rewrite eq_cons_iff.
-  Qed.
+Lemma eq_app_iff {A B C} : (A ++ B) ≡ (A ++ C) <-> B ≡ C.
+Proof.
+  elim: A.
+    done.
+  move=> a A IH /=.
+  by rewrite eq_cons_iff.
+Qed.
 
-  Lemma eq_length {A B} : A ≡ B -> length A = length B.
-    elim /(measure_ind (@length nat)) : A B.
-    case.
-      by move=> _ B /eq_nilE ->.
-    move=> a A IH B /copy [/eq_in_iff /(_ a) /iffLR]. apply: unnest.
-      by left.
-    move /(@in_split _ _) => [B1 [B2 ->]].
-    under (eq_lr eq_refl (B' := a :: (B1 ++ B2))).
-      by eq_trivial.
-    move /eq_cons_iff. move /IH. apply: unnest.
-      done.
-    rewrite ? app_length => /=. by lia.
-  Qed.
+Lemma eq_length {A B} : A ≡ B -> length A = length B.
+  elim /(measure_ind (@length nat)) : A B.
+  case.
+    by move=> _ B /eq_nilE ->.
+  move=> a A IH B /copy [/eq_in_iff /(_ a) /iffLR]. apply: unnest.
+    by left.
+  move /(@in_split _ _) => [B1 [B2 ->]].
+  under (eq_lr eq_refl (B' := a :: (B1 ++ B2))).
+    by eq_trivial.
+  move /eq_cons_iff. move /IH. apply: unnest.
+    done.
+  rewrite ? app_length => /=. by lia.
+Qed.
 
-  Lemma eq_repeatE {a A n} : repeat a n ≡ A -> A = repeat a n.
-  Proof.
-    move=> /copy [/eq_length]. rewrite repeat_length => HlA.
-    move /eq_Forall_iff /(_ (fun c => a = c)) /iffLR. apply: unnest.
-      clear. elim: n.
-        by constructor.
-      firstorder (by constructor).
-    subst n.
-    elim: A.
-      done.
-    move=> b A IH /Forall_cons_iff [<-] /IH -> /=.
-    by rewrite repeat_length.
-  Qed.
+Lemma eq_repeatE {a A n} : repeat a n ≡ A -> A = repeat a n.
+Proof.
+  move=> /copy [/eq_length]. rewrite repeat_length => HlA.
+  move /eq_Forall_iff /(_ (fun c => a = c)) /iffLR. apply: unnest.
+    clear. elim: n.
+      by constructor.
+    firstorder (by constructor).
+  subst n.
+  elim: A.
+    done.
+  move=> b A IH /Forall_cons_iff [<-] /IH -> /=.
+  by rewrite repeat_length.
+Qed.
 
-  Lemma eq_singletonE {a A} : [a] ≡ A -> A = [a].
-  Proof.
-    have -> : [a] = repeat a 1 by done.
-    by move /eq_repeatE.
-  Qed.
+Lemma eq_singletonE {a A} : [a] ≡ A -> A = [a].
+Proof.
+  have -> : [a] = repeat a 1 by done.
+  by move /eq_repeatE.
+Qed.
 
 Lemma eq_mapE {A} : map S A ≡ A -> A = [].
 Proof.
@@ -317,296 +349,444 @@ Proof.
   move /HA. by lia.
 Qed.
 
+(* interpret a multiset as a polynomial at p *)
+Section EvalPolynomial.
 
-(* mset facts *)
-Lemma try_remove_in {a A} : In a A -> exists B, mset_try_remove a A = Some B /\ A ≡ (a :: B).
+(* interpret a multiset as a polynomial at p *)
+Definition eval p A := fold_right plus 0 (map (fun n => Nat.pow p n) A).
+
+Lemma evalP {p A}: eval p A = fold_right plus 0 (map (fun n => Nat.pow p n) A).
+Proof. done. Qed.
+
+Lemma eval_consP {p a A} : eval p (a :: A) = p^a + eval p A.
+Proof. done. Qed.
+
+Lemma eval_singletonP {p a} : eval p [a] = p^a.
+Proof. cbn. by lia. Qed.
+
+Lemma eval_appP {p A B} : eval p (A ++ B) = eval p A + eval p B.
 Proof.
   elim: A.
     done.
-  move=> b A IH. rewrite in_cons_iff.
-  case: (Nat.eq_dec b a).
-    move=> ? ?. subst b. exists A. split.
-      rewrite /mset_try_remove. by rewrite Nat.eqb_refl.
-    done.
-  move=> ?. case.
-    done.
-  move /IH => [B [HaB HAB]]. exists (b :: B). split.
-    rewrite /mset_try_remove -/mset_try_remove. 
-    rewrite (iffRL (Nat.eqb_neq a b) (ltac:(lia))).
-    by rewrite HaB.
-  under (eq_lr eq_refl (B' := b :: (a :: B))).
-    by eq_trivial.
-  rewrite -/(mset_eq _ _). by apply /eq_cons_iff.
+  move=> a A IH /=. rewrite ? eval_consP. by lia.
 Qed.
 
-Lemma try_remove_not_in {a A} : not (In a A) -> mset_try_remove a A = None.
+Definition eval_norm := (@eval_appP, @eval_singletonP, @eval_consP).
+
+Lemma eval_nat {p A} : Forall (fun a => 0 = a) A -> eval p A = length A.
 Proof.
   elim: A.
     done.
-  move=> b A IH. rewrite in_cons_iff.
-  rewrite /mset_try_remove -/mset_try_remove.  
-  move /Decidable.not_or => [? /IH ->].
-  by rewrite (iffRL (Nat.eqb_neq a b) (ltac:(lia))).
+  move=> a A IH. rewrite ? Forall_norm ? eval_consP /length - /(length _).
+  by move=> [<- /IH ->].
 Qed.
 
-Lemma mset_intersectP {A B c} : 
-  (count_occ Nat.eq_dec (mset_intersect A B) c) = min (count_occ Nat.eq_dec A c) (count_occ Nat.eq_dec B c).
+Lemma eval_monotone {p q A} : p < q -> eval p A < eval q A \/ Forall (fun a => 0 = a) A.
+Proof.
+  move=> ?. elim: A.
+    by right.
+  case.
+    move=> A IH. rewrite ? eval_consP ? Forall_norm => /=.
+    case: IH=> IH.
+      left. by apply: lt_n_S.
+    by right.
+  move=> a A IH. left. rewrite ? eval_consP.
+  have ? := Nat.pow_lt_mono_l p q (S a) ltac:(done) ltac:(done).
+  case: IH.
+    by lia.
+  move /eval_nat => H. rewrite ? H. by lia.
+Qed.
+
+(* a non-increasing polynomial is degenerate *)
+Lemma eval_nat_spec {p q A} : p < q -> eval p A = eval q A -> Forall (fun a => 0 = a) A.
+Proof.
+  move /eval_monotone => /(_ A). case.
+    by lia.
+  done.
+Qed.
+
+Lemma eval_map {p A} : eval p (map S A) = p * eval p A.
+Proof.
+  elim: A.
+    done.
+  move=> a A IH. rewrite /map -/(map _ _) ? eval_consP IH.
+  rewrite /Nat.pow -/Nat.pow.
+  by nia.
+Qed.
+
+Lemma eval_eq {p A B} : A ≡ B -> eval p A = eval p B.
 Proof.
   elim: A B.
-    done.
-  move=> a A IH B. case: (in_dec Nat.eq_dec a B).
-    move /try_remove_in => [B' [HBB' /(_ c) ->]].
-    rewrite /mset_intersect -/mset_intersect HBB' /=.
-    case: (Nat.eq_dec a c)=> ?; rewrite IH; by lia.
-  rewrite /mset_intersect -/mset_intersect. move=> /copy [/try_remove_not_in -> ?].
-  rewrite IH => /=. case: (Nat.eq_dec a c)=> ?; first last.
-    done.
-  subst a. have -> := iffLR (count_occ_not_In Nat.eq_dec _ _) ltac:(eassumption).
-  by lia.
+    by move=> B /eq_nilE ->.
+  move => a A IH B /copy [/eq_in_iff /(_ a) /iffLR]. apply: unnest.
+    by left.
+  move /(@in_split _ _) => [B1 [B2 ->]].
+  under (eq_lr eq_refl (B' := a :: (B1 ++ B2))).
+    by eq_trivial.
+  move /eq_cons_iff /IH. rewrite ? eval_norm.
+  move=> ->. by lia.
 Qed.
 
-Lemma in_intersectI {a A B} : In a A -> In a B -> In a (mset_intersect A B).
-Proof.
-  rewrite ? (count_occ_In Nat.eq_dec) mset_intersectP.
-  by lia.
-Qed.
+End EvalPolynomial.
 
 (* 
   auxiliary soundness and completeness lemmas 
   for the reduction from H10UC to FMsetC
 *)
 
+(* nat constraints are only satisfied by multisets containing only zeroes *)
+Lemma nat_spec {n A B C} : 
+  (map S B) ++ A ≡ [n] ++ B ++ B ++ B ++ B ->
+  (map S (map S C)) ++ A ≡ [2*n] ++ C ++ C ++ C ++ C ->
+  Forall (fun a => 0 = a) A.
+Proof.
+  move=> /(eval_eq (p := 4)) + /(eval_eq (p := 2)).
+  rewrite ? eval_norm ? eval_map Nat.pow_mul_r.
+  move=> /= ? ?.
+  have : eval 2 A = eval 4 A by lia.
+  apply /eval_nat_spec.
+  by lia.
+Qed.
+
+Fixpoint tower m n :=
+  match n with 
+  | 0 => []
+  | S n => (tower m n) ++ (tower m n) ++ (tower m n) ++ (tower m n) ++ [m*n]
+  end.
+
+Lemma nat_sat {m n} :
+  (map (fun i => m + i) (tower m n)) ++ (repeat 0 (4^n)) ≡ [m*n] ++ (tower m n) ++ (tower m n) ++ (tower m n) ++ (tower m n).
+Proof.
+  elim: n.
+    by (have -> : m * 0 = 0 by nia).
+  move=> n IH /=. rewrite ? map_app ? repeat_add. cbn.
+  pose L := (map (fun i => m + i) (tower m n)) ++ (repeat 0 (4^n)).
+  pose R := [m*n] ++ (tower m n) ++ (tower m n) ++ (tower m n) ++ (tower m n).
+  have -> : m + m * n = m * (S n) by nia.
+  under (eq_lr (A' := (m * S n) :: (L ++ L ++ L ++ L)) (B' := (m * S n) :: (R ++ R ++ R ++ R))).
+    by eq_trivial.
+    by eq_trivial.
+  rewrite -/(mset_eq _ _).
+  apply /eq_cons_iff.
+  do 3 (apply /eq_appI; first done).
+  done.
+Qed.
+
 (* forces instance to be a sequence *)
 (* first constraint of encode bound *)
 (* type 1 constraint *)
-Lemma seq_spec A B : A ++ B ≡ [0] ++ (map S A) ->
-  exists n, A ≡ seq 0 n /\ B = [n].
+Lemma seq_spec2 {d A B} : A ++ B ≡ [0] ++ (map (fun i => (S d) + i) A) ->
+  exists n, A ≡ map (fun i => (S d) * i) (seq 0 n) /\ B = [(S d) * n].
 Proof.
   move /copy => [/eq_length + +].
   rewrite ? app_length map_length => /= H.
   have : length B = 1 by lia. clear H.
   move /singleton_length => [n ? Heq]. subst B. 
-  exists n. constructor => //.
+  exists (n / (S d)).
   move: n Heq.
   elim /(measure_ind (@length nat)) : A => A.
   case: (nil_or_ex_max A).
-    move=> -> _ n /= /eq_singletonE. by case=> <-.
+    move=> -> _ n /= /eq_singletonE. case=> <-. constructor.
+      done.
+    cbn. f_equal. by nia.
   move=> [m [+ Hm]].
   move /(in_split _ _) => [A1 [A2 ?]]. subst A.
   move=> IH n.
   move /copy => [H +].
-  have: n = 1+m.
+  have: n = (S d)+m.
     move : H.
-    move /eq_in_iff /(_ (1+m)) /iffRL.
+    move /eq_in_iff /(_ ((S d)+m)) /iffRL.
     apply: unnest. 
-      rewrite ? (in_app_iff, in_cons_iff, map_app, map_cons). by auto.
+      rewrite ? (in_app_iff, in_cons_iff, map_app, map_cons). by lia.
     rewrite in_app_iff. case.
       move: Hm => /Forall_forall. move=> + H. move /(_ _ H). by lia.
     rewrite /In /plus. by case.
   move=> ?. subst n.
-  under (eq_lr (A' := (1 + m) :: (A1 ++ A2) ++ [m]) (B' := (1 + m) :: 0 :: map S (A1 ++ A2))).
+  under (eq_lr (A' := ((S d) + m) :: (A1 ++ A2) ++ [m]) (B' := ((S d) + m) :: 0 :: map (fun i : nat => S (d + i)) (A1 ++ A2))).
   all: rewrite -/(mset_eq _ _).
     by eq_trivial.
     rewrite ? map_app map_cons /plus. by eq_trivial.
   move /eq_cons_iff /IH.
   apply: unnest.
     rewrite ? app_length => /=. by lia.
-  move => ?.
-  under (eq_lr (A' := m :: (A1 ++ A2)) (B' := m :: (seq 0 m))).
+  move=> [IHA1A2].
+  case. rewrite  -/(Nat.div m (S d)) - ? /(mult (S d) _).
+  have -> : S d + m = 1 * S d + m by lia.
+  rewrite Nat.div_add_l.
+    by lia.
+  rewrite seq_last map_app map_cons.
+  have -> : S d * (1 + m / S d) = S d + S d * (m / S d) by lia.
+  move=> IHm. rewrite  -/(Nat.div m (S d)) - ? /(mult (S d) _).
+  rewrite /plus -/plus.  
+  rewrite - ? IHm.
+  constructor; first last.
+    f_equal. by lia.
+  under (eq_lr (A' := m :: (A1 ++ A2)) (B' := m :: map (fun i : nat => i + d * i) (seq 0 (m / S d)))).
   all: rewrite -/(mset_eq _ _).
     by eq_trivial.
-    rewrite seq_last /plus. by eq_trivial.
+    by eq_trivial.
   by apply /eq_cons_iff.
 Qed.
 
 (* type 1 constraint satisfied by any sequence *)
-Lemma seq_sat n : (seq 0 n) ++ [n] ≡ [0] ++ (map S (seq 0 n)).
+Lemma seq_sat2 {d n} : 
+  let A n := map (fun i => (S d) * i) (seq 0 n) in
+  (A n) ++ [(S d) * n] ≡ [0] ++ (map (fun i => (S d) + i) (A n)).
 Proof.
-  rewrite seq_shift - seq_last. 
-  by apply: eq_refl.
+  move=> A. elim: n.
+    apply /eq_eq. cbn. f_equal. by nia.
+  move=> n IH.
+  rewrite /A seq_last ? map_app -/(A n) /plus -/plus.
+  rewrite /(map _ [n]) /(map _ [S d * n]).
+  have -> : S (d + S d * n) = S d * S n by lia.
+  under map_ext => i. rewrite -/(plus (S d) i). over.
+  rewrite -/(mset_eq _ _).
+  under (eq_lr 
+    (A' := S d * S n :: (A n ++ [S d * n])) 
+    (B' := S d * S n :: ([0] ++ map [eta Init.Nat.add (S d)] (A n)))).
+    by eq_trivial.
+    by eq_trivial.
+  rewrite -/(mset_eq _ _).
+  by apply /eq_cons_iff.
 Qed.
 
-(* auxiliary lemma for nat_spec *)
-Lemma nat_spec_aux n A B C : C ++ (n :: A) ≡ B ++ (map S A) -> 
-  Forall (fun b => b = 0 \/ n < b) B -> 
-  exists A' B', A ≡ (seq 0 n) ++ A' /\ B ≡ 0 :: B' /\ C ++ A' ≡ B' ++ (map S A').
+Lemma seq_sat1 {n} : 
+  (seq 0 n) ++ [n] ≡ [0] ++ (map S (seq 0 n)).
 Proof.
-  elim: n A B.
-    move=> A B /copy [/eq_in_iff /(_ 0) /iffLR].
-    apply: unnest. 
-      apply /in_app_iff. right. by firstorder done. 
-    move /in_app_iff. case; first last.
-      move /in_map_iff=> [? [? ?]]. by lia.
-    move /(@in_split _ _) => [B1 [B2 ->]].
-    under (eq_lr _ _ (A' := 0 :: (C ++ A)) (B' := 0 :: ((B1 ++  B2) ++ map S A))).
+  have -> : S = (fun i => (S 0) + i) by done.
+  have -> : seq 0 n = map (fun i => (S 0) * i) (seq 0 n).
+    elim: n.
+      done.
+    move=> n IH. rewrite seq_last map_app - IH => /=.
+    by rewrite Nat.add_0_r.
+  have -> : [n] = [1*n] by f_equal; lia.
+  by apply: seq_sat2.
+Qed.
+
+Lemma unify_spec {A m n} : A ++ (map (fun i => 2 * i) (seq 0 m)) ≡ (seq 0 n) ++ map S A ->
+  n = m.
+Proof.
+  move /eq_length.
+  rewrite ? app_length ? map_length ? seq_length.
+  by lia.
+Qed.
+
+Lemma unify_sat_aux {B n} : 
+  Forall2 (fun i j => i >= j) B (seq 0 n) -> {A | A ++ B ≡ (seq 0 n) ++ map S A}.
+Proof.
+  elim /(induction_ltof1 _ (fold_right (fun x y => S (x + y)) 0)) : B n.
+  rewrite /ltof.
+  move=> B.
+  case (list_eq_dec Nat.eq_dec B []).
+    move=> -> ? ? /Forall2_nil_lE ->. by exists [].
+  move /exists_last=> [C [a HC]]. subst B. move => IH. case.
+    move=> /Forall2_nil_rE /app_eq_nil. by case.
+  move=> n. rewrite seq_last /plus. move /Forall2_lastP => [HC Ha].
+  have := gt_eq_gt_dec n a. case; first case; first last.
+    move=> ?. exfalso. by lia.
+    move=> ?. subst a. move: (IH C).
+    apply: unnest_t.
+      clear. elim: C=> /= *; by lia. 
+    move /(_ _ ltac:(eassumption)) => [A HA]. exists A.
+    under (eq_lr (A' := n :: (A ++ C)) (B' := n :: (seq 0 n ++ map S A))).
       by eq_trivial.
       by eq_trivial.
-    move /eq_cons_iff => H _. exists A, (B1 ++ B2).
-    split=> //. split=> //.
+    rewrite -/(mset_eq _ _). by apply /eq_cons_iff.
+  move=> ?.
+  have HaSPa : a = S (Nat.pred a) by lia.
+  move: (IH (C ++ [Nat.pred a])).
+  apply: unnest_t.
+    move: HaSPa. clear. elim: C => /= [|? ? IH /IH] ?; by lia.
+  move /(_ (S n)). apply: unnest_t.
+    rewrite seq_last /plus. apply /Forall2_lastP. constructor; by [|lia].
+  move=> [A HA]. exists ((Nat.pred a) :: A).
+  rewrite -seq_last /(map) -/(map _ _) - HaSPa.
+  under (eq_lr (A' := a :: (A ++ C ++ [Nat.pred a])) (B' := a :: (seq 0 (S n) ++ map S A))).
     by eq_trivial.
-  move=> n IH A B /copy [/eq_in_iff /(_ (S n)) /iffLR].
-  apply: unnest. 
-    apply /in_app_iff. right. by firstorder done.
-  move /in_app_iff. case.
-    move=> H _ /Forall_forall => /(_ _ H). by lia.
-  move /in_map_iff=> [n' [+ +]]. case=> ?. subst n'.
-  move /(@in_split _ _) => [A1 [A2 ?]]. subst A.
-  under (eq_lr (A' := S n :: (C ++ (n :: (A1 ++ A2)))) (B' := S n :: (B ++ map S (A1 ++ A2)))).
     by eq_trivial.
-    move=> c. rewrite ? map_app map_cons. move: c. by eq_trivial.
-  move /eq_cons_iff => /IH + HB. apply: unnest.
-    move: HB. apply /Forall_impl. move=> ?. by lia.
-  move=> [A' [B' [? [? ?]]]]. exists A', B'.
-  split=> //.
-  rewrite seq_last.
-  under (eq_lr (A' := n :: (A1 ++ A2)) (B' := n :: (seq 0 n ++ A'))).
-    by eq_trivial.
-    rewrite /plus. by eq_trivial.
   rewrite -/(mset_eq _ _). by apply /eq_cons_iff.
 Qed.
 
-
-(* forces elements of A to be either zero or large enough *)
-Lemma bound_spec {n A B C} : C ≡ seq 0 n -> (mset_intersect C A) ++ B ≡ [0] -> Forall (fun a => a = 0 \/ n <= a) A.
+Definition unify_sat n :
+  {A | A ++ (map (fun i => 2*i) (seq 0 n)) ≡ (seq 0 n) ++ map S A}.
 Proof.
-  move => HC /eq_in_iff => Heq.
-  case: (Forall_dec (fun a : nat => a = 0 \/ n <= a) _ A) => //.
-    case. 
-      left; by left.
-    move=> m.
-    case: (le_lt_dec n (S m)) => ?.
-      left; by right.
-    right. by lia.
-  rewrite <- Exists_Forall_neg; first last.
-    move=> ?. by lia.
-  move/Exists_exists => [a [? ?]]. exfalso.
-  have ?: 0 <> a by lia. have: a < n by lia.
-  move=> ?.
-  have: 0 <= a < 0 + n by lia.
-  move /in_seq => H. move: HC => /eq_in_iff /(_ a) /iffRL /(_ H){H} => ?.
-  have H: In a (mset_intersect C A) by apply: in_intersectI.
-  move: (Heq a) => /iffLR. rewrite in_app_iff.
-  apply: unnest. by left.
-  by case.
+  apply: unify_sat_aux. elim: n.
+    by constructor.
+  move=> n IH. rewrite ? seq_last map_app. apply: Forall2_app.
+    done.
+  constructor.
+    by lia.
+  done.
 Qed.
 
-Lemma bound_sat_aux {m n l} : m > 0 -> mset_intersect (seq m n) (repeat 0 l) = [].
-Proof.
-  elim: n m l.
-    by done.
-  move=> n IH m l Hm. rewrite /seq -/seq /mset_intersect -/mset_intersect.
-  have: mset_try_remove m (repeat 0 l) = None.
-    elim: l=> //.
-    move=> a IH' /=.
-    rewrite (iffRL (Nat.eqb_neq m 0) (ltac:(lia))).
-    by rewrite IH'.
-  move=> ->. apply /IH. by lia.
+(* embed nat^3 into nat to provide fresh variables *)
+Definition embed '(x, y, z) := NatNat.nat2_to_nat (NatNat.nat2_to_nat (x, y), z).
+Definition unembed n := let (xy, z) := NatNat.nat_to_nat2 n in
+  (NatNat.nat_to_nat2 xy, z).
+
+
+Lemma embed_unembed {xyz} : unembed (embed xyz) = xyz.
+Proof. 
+  case: xyz. case. move=> >.
+  by rewrite /embed /unembed ? NatNat.nat_nat2_cancel.
 Qed.
 
-(* bound constraints are satisfied *)
-Lemma bound_sat {n} : (mset_intersect (seq 0 n) (repeat 0 n)) ++ (if n is 0 then [0] else []) ≡ [0].
-Proof.
-  case: n.
-    by done.
-  move=> n /=. rewrite app_nil_r. apply /eq_cons_iff.
-  apply: eq_eq. by apply: bound_sat_aux.
-Qed.
+Opaque embed unembed.
 
-(* forces B to be a n zeroes and A to be of length in proportion to n squared *)
-Lemma nat_spec n A B : (seq 0 n) ++ A ≡ B ++ (map S A) -> 
-  Forall (fun b => b = 0 \/ n <= b) B -> B = repeat 0 n /\ length A + length A + n = n * n.
+Definition encode_bound (x: nat): FMsetC_PROBLEM :=
+  let X n := embed (x, n, 0) in
+    [
+      ((X 1) ⊍ (X 2), •0 ⊍ (h (X 1))); (* X 1 = [0..n-1], X 2 = [n] *)
+      ((X 3) ⊍ (X 4), •0 ⊍ (h (h (X 3)))); (* X 3 = [0,2,..2*(m-1)], X 4 = [2*m] *)
+      ((X 5) ⊍ (X 3), (X 1) ⊍ (h (X 5))); (* n = m *)
+      ((h (X 6)) ⊍ (X 0), (X 2) ⊍ ((X 6) ⊍ ((X 6) ⊍ ((X 6) ⊍ (X 6)))));
+      ((h (h (X 7))) ⊍ (X 0), (X 4) ⊍ ((X 7) ⊍ ((X 7) ⊍ ((X 7) ⊍ (X 7))))) (* X 0 = [0..0] of length 2^n *)
+    ].
+
+Definition encode_bound_spec {φ x} : mset_sat φ (encode_bound x) -> 
+  Forall (fun a => 0 = a) (φ (embed (x, 0, 0))).
 Proof.
-  elim: n A B.
-    move=> A B /copy [/eq_length] /=. rewrite ? app_length map_length.
-    move=> ?. have: length B = 0 by lia. move /length_zero_iff_nil.
-    move=> ->. rewrite /app. by move /eq_symm /eq_mapE => ->.
-  move=> n IH A B. rewrite seq_last /plus -/plus.
-  under (eq_lr _ eq_refl (A' := seq 0 n ++ (n :: A))).
-    by eq_trivial.
-  move /nat_spec_aux => + HB. apply: unnest.
-    move: HB. apply /Forall_impl => ?. by lia.
-  move=> [A' [B' [HA' [HB']]]]. move /IH.
-  apply: unnest.
-    move: HB' => /eq_Forall_iff. move /(_ (fun b : nat => b = 0 \/ n <= b)) /iffLR.
-    apply: unnest.
-      move: HB. apply /Forall_impl. move=> ?. by lia.
-    move /Forall_cons_iff=> [_].
-    apply /Forall_impl. move=> ?. by lia.
-  move=> [? ?]. subst B'. move : HB'. rewrite -/(repeat 0 (S n)).
-  move /eq_symm /eq_repeatE => ?. split=> //.
-  move: HA' => /eq_length. rewrite app_length seq_length. by lia. 
+  rewrite /encode_bound /mset_sat ? Forall_norm /mset_sem.
+  have -> (A) : map S (map S A) = map (fun i => (S 1) + i) A.
+    by rewrite map_map.
+  have -> : map S = map [eta Nat.add 1] by done.
+
+  move=> [/seq_spec2 [n [/eq_length Hn ->]]].
+  move=> [/seq_spec2 [m [/eq_length Hm ->]]].
+  move=> [/eq_length]. rewrite ? app_length Hn Hm ? map_length ? seq_length => ?.
+  have ? : n = m by lia. subst m. clear.
+  have -> : [eta Nat.add 1] = S by done.
+  have -> : 1 * n = n by lia.
+  move=> [H1 H2]. by apply: nat_spec.
 Qed.
 
 (* [0] ++ [0,1] ++ [0,1,2] ++ ...*)
 Definition pyramid n := flat_map (seq 0) (seq 0 n).
 
-(* nat containstraints are satisfied using pyramid *)
-Lemma nat_sat {n}: (seq 0 n) ++ (pyramid n) ≡ (repeat 0 n) ++ (map S (pyramid n)).
+(* from a H10UC valuation φ construct a valuation for FMsetC *)
+Definition construct_valuation (φ: nat -> nat) (n: nat): list nat :=
+  match unembed n with
+  | (x, 0, 0) => repeat 0 (4^(φ x))
+  | (x, 1, 0) => seq 0 (φ x)
+  | (x, 2, 0) => [(φ x)]
+  | (x, 3, 0) => map (fun i => 2*i) (seq 0 (φ x))
+  | (x, 4, 0) => [2*(φ x)]
+  | (x, 5, 0) => proj1_sig (unify_sat (φ x))
+  | (x, 6, 0) => tower 1 (φ x)
+  | (x, 7, 0) => tower 2 (φ x)
+  | (x, 0, 1) => repeat 0 (φ x)
+  | (x, 1, 1) => repeat 0 (length (pyramid (φ x)))
+  | (x, 2, 1) => repeat 0 (4^(φ x) - (φ x))
+  | (x, 3, 1) => repeat 0 (4^(φ x) - (length (pyramid (φ x))))
+  | (x, 4, 1) => seq 0 (φ x)
+  | (x, 5, 1) => [(φ x)]
+  | (x, 6, 1) => pyramid (φ x)
+  | (x, 7, 1) => flat_map pyramid (seq 0 (φ x))
+  | _ => []
+  end.
+
+
+Lemma encode_bound_sat {φ x} : 
+  mset_sat (construct_valuation φ) (encode_bound x).
 Proof.
-  elim: n.
-    by done.
-  move=> n IH.
-  rewrite /pyramid ? seq_last ? /plus. 
-  rewrite ? flat_map_concat_map map_app concat_app.
-  rewrite - ? flat_map_concat_map -/(pyramid _).
-  rewrite map_app /flat_map ? app_nil_r /repeat -/(repeat _ n).
-  rewrite - seq_last seq_shift.
-  under (eq_lr 
-    (A' := seq 0 (S n) ++ (seq 0 n ++ pyramid n)) 
-    (B' := (0 :: seq 1 n) ++ (repeat 0 n ++ map S (pyramid n)))).
-    by eq_trivial.
-    by eq_trivial.
-  rewrite -/(mset_eq _ _). by apply /eq_app_iff.
+  rewrite /encode_bound /mset_sat ? Forall_norm /mset_sem.
+  rewrite /construct_valuation ? embed_unembed.
+  pose A d n := map (fun i => (S d) * i) (seq 0 n).
+  constructor.
+    by apply: seq_sat1.
+  constructor.
+    have -> (X) : map S (map S X) = map (fun i => 2+i) X by rewrite map_map.
+    by apply: seq_sat2.
+  constructor.
+    apply: proj2_sig (unify_sat _).
+  constructor.
+    have -> (n): [n] = [1*n] by f_equal; lia.
+    by apply: nat_sat.
+  rewrite map_map.
+  by apply: nat_sat.
 Qed.
-
-(* embedding provides fresh auxiliary variables *)
-Definition embed xy := NatNat.nat2_to_nat xy.
-Definition unembed n := NatNat.nat_to_nat2 n.
-Opaque embed unembed.
-
-Lemma embed_unembed {xy} : unembed (embed xy) = xy.
-Proof. apply: NatNat.nat_nat2_cancel. Qed.
 
 (* each n : nat is represented by a multiset containing n zeroes *)
 Definition encode_nat (x: nat) : FMsetC_PROBLEM :=
-  let X := embed (x, 0) in
-  let XX := embed (x, 1) in
-  let Ax := embed (x, 2) in
-  let Bx := embed (x, 3) in
-  let Cx := embed (x, 4) in
-  let Dx := embed (x, 5) in
-  let Ex := embed (x, 6) in
+  let X n := embed (x, n, 1) in
     [
-      (Ax ⊍ Bx, •[0] ⊍ (h Ax)); (* Ax = seq 0 (φ x) *)
-      ((Ax ⩀ X) ⊍ Cx, •[0]); (* bounding constraints *)
-      (Ax ⊍ Dx, X ⊍ (h Dx)); (* X is solved by n zeroes *)
-      (Dx ⊍ Ex, XX ⊍ (h Ex)) (* XX is solved by sets of size proportional to the squared size of X *)
+      (X 0 ⊍ X 2, mset_term_var (embed (x, 0, 0))); (* X 0 = [0..0] *)
+      (X 1 ⊍ X 3, mset_term_var (embed (x, 0, 0))); (* X 1 = [0..0] *)
+      (X 4 ⊍ X 5, •0 ⊍ (h (X 4))); (* X 4 = [0..m-1], X 5 = [m]*)
+      (X 4 ⊍ X 6, X 0 ⊍ (h (X 6))); (* m = length (X 0), length (X 6) ~ m * m *)
+      (X 6 ⊍ X 7, X 1 ⊍ (h (X 7))) (* length X 1 ~ m * m *)
     ].
 
-Lemma encode_nat_spec {φ x} : mset_sat φ (encode_nat x) -> 
-  length (φ (embed (x, 1))) + length (φ (embed (x, 1))) + length (φ (embed (x, 0))) = 
-    length (φ (embed (x, 0))) * length (φ (embed (x, 0))).
+(* auxiliary lemma for square_spec *)
+Lemma square_spec_aux {n m A C} : C ++ (n :: A) ≡ (repeat 0 (S m)) ++ (map S A) -> 
+exists A', A ≡ (seq 0 n) ++ A' /\ C ++ A' ≡ (repeat 0 m) ++ (map S A').
 Proof.
+elim: n A.
+  move=> A. rewrite /repeat -/(repeat _).
+  under (eq_lr (A' := 0 :: (C ++ A)) (B' := 0 :: ((repeat 0 m) ++ map S A))).
+    by eq_trivial.
+    by eq_trivial.
+  move /eq_cons_iff=> ?. exists A. by constructor.
+move=> n IH A /copy [/eq_in_iff /(_ (S n)) /iffLR].
+apply: unnest. 
+  apply /in_app_iff. right. by left.
+move /in_app_iff. case.
+  by move /(@repeat_spec _ _ _ _).
+move /in_map_iff=> [n' [+ +]]. case=> ?. subst n'.
+move /(@in_split _ _) => [A1 [A2 ?]]. subst A.
+
+under (eq_lr (A' := S n :: (C ++ (n :: (A1 ++ A2)))) (B' := S n :: ((repeat 0 (S m)) ++ map S (A1 ++ A2)))).
+  by eq_trivial.
+  move=> c. rewrite ? map_app map_cons. move: c. by eq_trivial.
+move /eq_cons_iff => /IH [A' [? ?]].
+exists A'. constructor.
+  rewrite seq_last.
+  under (eq_lr (A' := n :: (A1 ++ A2)) (B' := n :: (seq 0 n ++ A'))).
+    by eq_trivial.
+    rewrite /plus. by eq_trivial.
+  rewrite -/(mset_eq _ _). by apply /eq_cons_iff.
+done.
+Qed.
+
+(* forces B to be a n zeroes and A to be of length in proportion to n squared *)
+Lemma square_spec {n A} : (seq 0 n) ++ A ≡ (repeat 0 n) ++ (map S A) -> 
+length A + length A + n = n * n.
+Proof.
+elim: n A.
+  move=> A /=. by move=> /eq_symm /eq_mapE ->.
+move=> n IH A. rewrite seq_last /plus -/plus.
+under (eq_lr _ eq_refl (A' := seq 0 n ++ (n :: A))).
+  by eq_trivial.
+move /square_spec_aux => [A' [/eq_length + /IH]].
+rewrite app_length seq_length. by lia. 
+Qed.
+
+(* if encode bound is satisfied, then there is a square relationship on length of solutions *)
+Lemma encode_nat_spec {φ x} : mset_sat φ (encode_bound x) -> mset_sat φ (encode_nat x) -> 
+  length (φ (embed (x, 1, 1))) + length (φ (embed (x, 1, 1))) + length (φ (embed (x, 0, 1))) = 
+    length (φ (embed (x, 0, 1))) * length (φ (embed (x, 0, 1))).
+Proof.
+  move /encode_bound_spec.
   rewrite /mset_sat /encode_nat.
   rewrite ? Forall_norm /mset_sem.
-  move=> [+ [+ [+]]].
-  move: (φ (embed (x, 0)))=> X. move: (φ (embed (x, 1)))=> XX. 
-  move: (φ (embed (x, 2)))=> A. move: (φ (embed (x, 3)))=> B.
-  move: (φ (embed (x, 4)))=> C. move: (φ (embed (x, 5)))=> D. 
-  move: (φ (embed (x, 6)))=> E.
-
-  move /seq_spec => [n [Hseq _]].
-  move /bound_spec => /(_ _ ltac:(eassumption)) HX.
-  under (eq_lr _ eq_refl (A' := (seq 0 n) ++ D)).
-    rewrite -/(mset_eq _ _).
-    under (eq_lr (A' := D ++ A) (B' := D ++ seq 0 n)).
-      by eq_trivial.
-      by eq_trivial.
-    rewrite -/(mset_eq _ _). by apply /eq_app_iff.
-  move /nat_spec => /(_ ltac:(assumption)).
-  move=> [/copy [+ ?] ?]. 
-  move /(f_equal (@length nat)). rewrite repeat_length => ?.
-  move /eq_length. rewrite ? app_length map_length.
+  pose X n := φ (embed (x, n, 1)). rewrite - ? /(X _).
+  move=> H.
+  move=> [/eq_Forall_iff /(_ [eta eq 0]) /iffRL /(_ H)].
+  rewrite Forall_norm=> [[HX0 _]].
+  move=> [/eq_Forall_iff /(_ [eta eq 0]) /iffRL /(_ H)].
+  rewrite Forall_norm=> [[? _]].
+  have -> : map S (X 4) = map [eta Init.Nat.add 1] (X 4) by done.
+  move=> [/seq_spec2 [n]].
+  have -> : map [eta Init.Nat.mul 1] (seq 0 n) = map id (seq 0 n).
+    under map_ext => i. have -> : 1*i = i by lia. over. done.
+  rewrite map_id => [[Hn _]].
+  move=> [/eq_symm /eq_trans] => /(_ ((seq 0 n) ++ X 6)). apply: unnest.
+    by apply: eq_appI.
+  move => HX6. have HlX0 : length (X 0) = n.
+    move: HX6 => /eq_length. rewrite ? app_length map_length seq_length. by lia.
+  move: HX6 => /eq_symm. have -> := Forall_repeat HX0. rewrite HlX0. 
+  move /square_spec => ?.
+  move /eq_length. rewrite ? app_length map_length repeat_length.
   by lia.
 Qed.
 
@@ -650,71 +830,83 @@ Proof.
   by apply: pyramid_shuffle.
 Qed.
 
-Definition encode_nat_vars φ x n : Prop :=
-  φ (embed (x, 0)) = repeat 0 n /\
-  φ (embed (x, 1)) = repeat 0 (length (pyramid n)) /\
-  φ (embed (x, 2)) = seq 0 n /\
-  φ (embed (x, 3)) = [n] /\
-  φ (embed (x, 4)) = (if n is 0 then [0] else []) /\
-  φ (embed (x, 5)) = pyramid n /\
-  φ (embed (x, 6)) = flat_map pyramid (seq 0 n).
-
-Lemma encode_nat_sat {φ x n} : 
-  encode_nat_vars φ x n -> mset_sat φ (encode_nat x).
+Lemma pyramid_length n : n + length (pyramid n) <= 4 ^ n.
 Proof.
-  rewrite /encode_nat_vars /encode_nat /mset_sat ? Forall_norm /mset_sem.
-  do 6 (move=> [->]). move=> ->.
-  split. 
-    by apply: seq_sat.
-  split.
-    by apply: @bound_sat.
-  split.
-    by apply: nat_sat.
+  elim: n.
+    cbn. by lia.
+  move=> n IH. 
+  rewrite /pyramid seq_last /plus -/plus flat_map_concat_map map_app concat_app app_length.
+  rewrite -flat_map_concat_map -/(pyramid _).
+  rewrite /map /concat app_length seq_length. move=> /=.
+  case: n IH.
+    rewrite /Nat.pow. by lia.
+  move=> n. have := Nat.pow_gt_1 4 (S n) ltac:(lia) ltac:(lia).
+    by lia.
+Qed.
+
+Lemma encode_nat_sat {φ x} : 
+  mset_sat (construct_valuation φ) (encode_nat x).
+Proof.
+  rewrite /encode_nat /mset_sat ? Forall_norm /mset_sem.
+  rewrite /construct_valuation ? embed_unembed.
+  constructor.
+    rewrite - repeat_add. apply: eq_eq. f_equal.
+    have := pyramid_length (φ x).
+    by lia.
+  constructor.
+    rewrite - repeat_add. apply: eq_eq. f_equal.
+    have := pyramid_length (φ x).
+    by lia.
+  constructor.
+    by apply: seq_sat1.
+  constructor.
+    by apply: pyramid_shuffle.
   by apply: encode_nat_sat_aux.
 Qed.
 
 (* represent constraints of shape 1 + x + y * y = z *)
 Definition encode_constraint x y z := 
+  encode_bound x ++ encode_bound y ++ encode_bound z ++ 
   encode_nat x ++ encode_nat y ++ encode_nat z ++ 
-  let x := embed (x, 0) in
-  let yy := embed (y, 1) in
-  let y := embed (y, 0) in
-  let z := embed (z, 0) in
-  [ (•[0] ⊍ x ⊍ yy ⊍ yy ⊍ y, mset_term_var z) ].
+  let x := embed (x, 0, 1) in
+  let yy := embed (y, 1, 1) in
+  let y := embed (y, 0, 1) in
+  let z := embed (z, 0, 1) in
+  [ (•0 ⊍ x ⊍ yy ⊍ yy ⊍ y, mset_term_var z) ].
 
 (* if mset constraint has a solution, then uniform diophantine constraint is satisfied *)
-Lemma encode_constraint_spec {φ x y z} : mset_sat φ (encode_constraint x y z) -> 
-  1 + length (φ (embed (x, 0))) + length(φ (embed (y, 0))) * length(φ (embed (y, 0))) = length(φ (embed (z, 0))).
+Lemma encode_constraint_spec {φ x y z} :  
+  mset_sat φ (encode_constraint x y z) -> 
+  1 + length (φ (embed (x, 0, 1))) + length(φ (embed (y, 0, 1))) * length(φ (embed (y, 0, 1))) = length(φ (embed (z, 0, 1))).
 Proof.
-  rewrite /encode_constraint /mset_sat. rewrite ? (Forall_app_iff).
-  move => [/encode_nat_spec ? [/encode_nat_spec ? [ /encode_nat_spec ?]]].
-  rewrite Forall_norm /mset_sem.
+  rewrite /encode_constraint /mset_sat. rewrite ? (Forall_app_iff). rewrite - ? /(mset_sat _ _).
+  move=> [Hx [Hy [Hz]]].
+  move=> [/(encode_nat_spec Hx) ? [/(encode_nat_spec Hy) ? [/(encode_nat_spec Hz) ?]]].
+  rewrite /mset_sat Forall_norm /mset_sem.
   move /eq_length. rewrite ? app_length.
   have -> : (length [0] = 1) by done.
   by lia.
 Qed.
 
 (* if uniform diophantine constraint is satisfied, then mset constraint has a solution *)
-Lemma encode_constraint_sat {φ x y z xn yn zn} : 
-  encode_nat_vars φ x xn -> encode_nat_vars φ y yn -> encode_nat_vars φ z zn ->
-  1 + xn + yn * yn = zn -> mset_sat φ (encode_constraint x y z).
+Lemma encode_constraint_sat {φ x y z} : 
+  1 + (φ x) + (φ y) * (φ y) = (φ z) -> mset_sat (construct_valuation φ) (encode_constraint x y z).
 Proof.
-  move=> /copy [/encode_nat_sat ? Hx].
-  move=> /copy [/encode_nat_sat ? Hy].
-  move=> /copy [/encode_nat_sat ? Hz].
-  rewrite /encode_constraint /mset_sat ? Forall_app_iff Forall_singleton_iff.
   move=> Hxyz.
-  do 3 (split; [done|]).
-  rewrite /mset_sem.
-  move: Hx Hy Hz. rewrite /encode_nat_vars. move=> [-> _] [-> [-> _]] [-> _].
+  rewrite /encode_constraint /mset_sat ? Forall_app_iff Forall_singleton_iff.
+  rewrite - ? /(mset_sat _ _).
+  do 3 (constructor; first by apply: encode_bound_sat).
+  do 3 (constructor; first by apply: encode_nat_sat).
+  rewrite /mset_sem /construct_valuation ? embed_unembed.
   have ->: [0] = repeat 0 1 by done.
   rewrite - ? repeat_add. apply: eq_eq.
-  f_equal. subst zn. clear. elim: yn.
+  f_equal. move: Hxyz=> <-. clear. elim: (φ y); clear.
     cbn. by lia.
-  move=> yn IH. rewrite /pyramid seq_last /(plus 0 _) flat_map_concat_map map_app concat_app.
+  move=> φy IH. rewrite /pyramid seq_last /(plus 0 _) flat_map_concat_map map_app concat_app.
   rewrite -flat_map_concat_map -/(pyramid _).
   cbn. rewrite ? app_length seq_length. cbn. by lia.
 Qed.
+
 
 (* encode a single H10UC constraint as a list of FMsetC constraints *)
 Definition encode_h10uc '(x, y, z) := encode_constraint x y z.
@@ -722,21 +914,10 @@ Definition encode_h10uc '(x, y, z) := encode_constraint x y z.
 (* many-one reduction from H10UC to FMsetC *)
 Theorem H10UC_to_FMsetC : H10UC_SAT ⪯ FMsetC_SAT.
 Proof.
-  exists (flat_map encode_h10uc).
+  exists (fun h10ucs => flat_map encode_h10uc h10ucs).
   move=> h10ucs. constructor.
   - move=> [φ Hφ]. 
-    pose ψ := (fun x => 
-      match unembed x with
-      | (x, 0) => repeat 0 (φ x)
-      | (x, 1) => repeat 0 (length (pyramid (φ x)))
-      | (x, 2) => seq 0 (φ x)
-      | (x, 3) => [(φ x)]
-      | (x, 4) =>  (if (φ x) is 0 then [0] else [])
-      | (x, 5) => pyramid (φ x)
-      | (x, 6) => flat_map pyramid (seq 0 (φ x))
-      | _ => []
-      end).
-    exists ψ.
+    exists (construct_valuation φ).
     elim: h10ucs Hφ.
       done.
     move=> [[x y] z] h10cs IH.
@@ -745,21 +926,10 @@ Proof.
     rewrite /flat_map -/(flat_map _) in_app_iff. case; first last.
       by apply /IH.
     rewrite /encode_h10uc.
-    have := @encode_constraint_sat ψ x y z (φ x) (φ y) (φ z).
-    apply: unnest.
-      rewrite /encode_nat_vars.
-      firstorder (by rewrite /ψ embed_unembed).
-    apply: unnest.
-      rewrite /encode_nat_vars.
-      firstorder (by rewrite /ψ embed_unembed).
-    apply: unnest.
-      rewrite /encode_nat_vars.
-      firstorder (by rewrite /ψ embed_unembed).
-    apply: unnest.
-      done.
-    rewrite /mset_sat Forall_forall. apply.
+    have := @encode_constraint_sat φ x y z ltac:(done).
+    rewrite /mset_sat Forall_forall. by apply.
   - move=> [φ]. rewrite - mset_satP /mset_sat. move=> Hφ.
-    pose ψ := (fun x => length (φ (embed (x, 0)))).
+    pose ψ := (fun x => length (φ (embed (x, 0, 1)))).
     exists ψ.
     rewrite - Forall_forall.
     elim: h10ucs Hφ.
@@ -771,6 +941,7 @@ Proof.
 Qed.
 
 Check H10UC_to_FMsetC.
+(*Print Assumptions H10UC_to_FMsetC.*)
 
 From Undecidability Require Import Problems.TM.
 From Undecidability Require Import Reductions.H10C_to_H10UC.
